progress

src/Framework/KnownAnnotate.v
@@ -5,672 +5,839 @@ From CertiCoq.Libraries Require Import maps_util.
 Import ListNotations.
 Require Import Lia.
 
-From Framework Require Import Util ANF0 ANF Refl0 Refl Annotate Erase.
+From Framework Require Import Util ANF0 ANF Annotate Erase.
 
 Module A0 := ANF0.
 Module A1 := ANF.
 
 (* Known Function Analysis With A Single Exposed Web Id *)
 
-Module M <: Annotate.
+(* Similar to CertiCoq's `Known_exp` *)
+Inductive known_fun (S : Ensemble var) : A0.exp -> Prop :=
+| Known_Ret :
+  forall x,
+    (~ x \in S) ->
+    known_fun S (A0.Eret x)
 
-  (* Similar to CertiCoq's `Known_exp` *)
-  Inductive known_exp (S : Ensemble var) : A0.exp -> Prop :=
-  | Known_Ret :
+| Known_App :
+  forall f ys,
+    (f \in S) ->
+    Disjoint _ (FromList ys) S ->
+    known_fun S (A0.Eapp f ys)
+
+| Known_LetApp :
+  forall x f ys e,
+    (f \in S) ->
+    (~ x \in S) -> (* intermediate result shouldn't be known fun *)
+    Disjoint _ (FromList ys) S ->
+    known_fun S e ->
+    known_fun S (A0.Eletapp x f ys e)
+
+| Known_Fun:
+  forall f xs e k,
+    (f \in S) ->
+    known_fun S e ->
+    known_fun S k ->
+    known_fun S (A0.Efun f xs e k)
+
+| Known_Constr :
+  forall x ys ct e,
+    (~ x \in S) -> (* constructors are not known functions, but they can still be known exp *)
+    Disjoint _ (FromList ys) S ->
+    known_fun S e ->
+    known_fun S (A0.Econstr x ct ys e)
+
+| Known_Proj :
+  forall x n y e,
+    (~ x \in S) ->
+    (~ y \in S) ->
+    known_fun S e ->
+    known_fun S (A0.Eproj x n y e)
+
+| Known_Case_nil:
+  forall x,
+    (~ x \in S) ->
+    known_fun S (A0.Ecase x [])
+
+| Known_Case_hd:
+  forall x c e ce,
+    (~ x \in S) ->
+    known_fun S e ->
+    known_fun S (A0.Ecase x ce) ->
+    known_fun S (A0.Ecase x ((c, e) :: ce)).
+
+Hint Constructors known_fun : core.
+
+Definition known_map := M.t web.
+
+Definition known_map_inv K :=
+  forall f w,
+    K ! f = Some w ->
+    ~ (w \in Exposed).
+
+(* Outline: *)
+(* 1. build `K : known_map` for every function identifiers (assume unique names) in the program with nonexposed web ids (Note it is not necessary to require them to be distinct though) *)
+(* 2. follow `escape_fun_exp` as in CertiCoq to filter `K` so that its domain satisfies `known_fun` *)
+(* 3. rewrite based on `K` [this is the main result we are establishing here] *)
+
+Parameter analyze : A0.exp -> known_map.
+
+Axiom analyze_sound :
+  forall (e : A0.exp),
+    let K := analyze e in
+    known_fun (Dom_map K) e /\
+    known_map_inv K.
+
+Parameter w0 : web.
+Axiom w0_exposed : w0 \in Exposed.
+Axiom Exposed_singleton : forall w, w \in Exposed -> w = w0.
+
+Theorem Exposed_nonempty : exists w, w \in Exposed.
+Proof. exists w0. apply w0_exposed. Qed.
+
+Section Spec.
+  Variable K : known_map.
+
+  (* Specification *)
+  Inductive trans_ (Γ : A0.vars) : A0.exp -> A1.exp -> Prop :=
+  | Trans_ret :
     forall x,
-      (~ x \in S) ->
-      known_exp S (A0.Eret x)
+      K ! x = None ->
+      (x \in Γ) ->
+      trans_ Γ (A0.Eret x) (A1.Eret x)
 
-  | Known_App :
-    forall f ys,
-      Disjoint _ (FromList ys) S ->
-      known_exp S (A0.Eapp f ys)
-
-  | Known_LetApp :
-    forall x f ys e,
-      Disjoint _ (FromList ys) S ->
-      known_exp S e ->
-      known_exp S (A0.Eletapp x f ys e)
-
-  | Known_Fun:
-    forall f xs e k,
-      known_exp S e ->
-      known_exp S k ->
-      known_exp S (A0.Efun f xs e k)
-
-  | Known_Constr :
-    forall x ys ct e,
-      Disjoint _ (FromList ys) S ->
-      known_exp S e ->
-      known_exp S (A0.Econstr x ct ys e)
-
-  | Known_Proj :
-    forall x n y e,
-      (~ y \in S) ->
-      known_exp S e ->
-      known_exp S (A0.Eproj x n y e)
-
-  | Known_Case_nil:
-    forall x,
-      known_exp S (A0.Ecase x [])
-
-  | Known_Case_hd:
-    forall x c e ce,
-      known_exp S e ->
-      known_exp S (A0.Ecase x ce) ->
-      known_exp S (A0.Ecase x ((c, e) :: ce)).
-
-  Hint Constructors known_exp : core.
-
-  Definition known_map := M.t web.
-
-  Definition known_map_inv K :=
-    forall f w,
+  | Trans_fun_known :
+    forall {f w xs e k e' k'},
       K ! f = Some w ->
-      ~ (w \in Exposed).
+      (~ w \in Exposed) ->
 
-  (* Outline: *)
-  (* 1. build `K : known_map` for every function identifiers (assume unique names) in the program with nonexposed web ids (Note it is not necessary to require them to be distinct though) *)
-  (* 2. follow `escape_fun_exp` as in CertiCoq to filter `K` so that its domain satisfies `known_exp` *)
-  (* 3. rewrite based on `K` [this is the main step we are focusing on here] *)
+      trans_ (FromList xs :|: (f |: Γ)) e e' ->
+      trans_ (f |: Γ) k k' ->
+      trans_ Γ (A0.Efun f xs e k) (A1.Efun f w xs e' k')
 
-  (* TODO: define `analyze` following `escape_fun_exp` in CertiCoq *)
-  Parameter analyze : A0.exp -> known_map.
+  | Trans_fun_unknown :
+    forall {f xs e k e' k'},
+      K ! f = None ->
 
-  Axiom analyze_sound :
-    forall (e : A0.exp),
-      let K := analyze e in
-      known_exp (Dom_map K) e /\
-      known_map_inv K.
+      trans_ (FromList xs :|: (f |: Γ)) e e' ->
+      trans_ (f |: Γ) k k' ->
+      trans_ Γ (A0.Efun f xs e k) (A1.Efun f w0 xs e' k')
 
-  Parameter w0 : web.
-  Axiom w0_exposed : w0 \in Exposed.
-  Axiom Exposed_singleton : forall w, w \in Exposed -> w = w0.
+  | Trans_app_known :
+    forall {f w xs},
+      K ! f = Some w ->
+      (~ w \in Exposed) ->
+      Disjoint _ (FromList xs) (Dom_map K) ->
 
-  Theorem Exposed_nonempty : exists w, w \in Exposed.
-  Proof. exists w0. apply w0_exposed. Qed.
+      (f \in Γ) ->
+      (FromList xs \subset Γ) ->
+      trans_ Γ (A0.Eapp f xs) (A1.Eapp f w xs)
 
-  Section Spec.
-    Variable K : known_map.
+  | Trans_app_unknown :
+    forall {f xs},
+      K ! f = None ->
+      Disjoint _ (FromList xs) (Dom_map K) ->
 
-    (* Specification *)
-    Inductive trans_ (Γ : A0.vars) : A0.exp -> A1.exp -> Prop :=
-    | Trans_ret :
-      forall x,
-        K ! x = None ->
+      (f \in Γ) ->
+      (FromList xs \subset Γ) ->
+      trans_ Γ (A0.Eapp f xs) (A1.Eapp f w0 xs)
 
-        (x \in Γ) ->
-        trans_ Γ (A0.Eret x) (A1.Eret x)
+  (* TODO: letapp *)
+  (* data webs are all exposed *)
 
-    | Trans_fun_known :
-      forall {f w xs e k e' k'},
-        K ! f = Some w ->
-        (~ w \in Exposed) ->
+  | Trans_constr :
+    forall {x t xs k k'},
+      Disjoint _ (FromList xs) (Dom_map K) ->
 
-        trans_ (FromList xs :|: (f |: Γ)) e e' ->
-        trans_ (f |: Γ) k k' ->
-        trans_ Γ (A0.Efun f xs e k) (A1.Efun f w xs e' k')
+      (FromList xs \subset Γ) ->
+      trans_ (x |: Γ) k k' ->
+      trans_ Γ (A0.Econstr x t xs k) (A1.Econstr x w0 t xs k')
 
-    | Trans_fun_unknown :
-      forall {f xs e k e' k'},
-        K ! f = None ->
+  | Trans_proj :
+    forall {x y k k' n},
+      K ! x = None ->
 
-        trans_ (FromList xs :|: (f |: Γ)) e e' ->
-        trans_ (f |: Γ) k k' ->
-        trans_ Γ (A0.Efun f xs e k) (A1.Efun f w0 xs e' k')
+      (y \in Γ) ->
+      trans_ (x |: Γ) k k' ->
+      trans_ Γ (A0.Eproj x n y k) (A1.Eproj x w0 n y k')
 
-    | Trans_app_known :
-      forall {f w xs},
-        K ! f = Some w ->
-        (~ w \in Exposed) ->
-        Disjoint _ (FromList xs) (Dom_map K) ->
+  | Trans_case_nil :
+    forall {x},
+      (x \in Γ) ->
+      trans_ Γ (A0.Ecase x []) (A1.Ecase x w0 [])
 
-        (f \in Γ) ->
-        (FromList xs \subset Γ) ->
-        trans_ Γ (A0.Eapp f xs) (A1.Eapp f w xs)
+  | Trans_case_cons :
+    forall {x e e' t cl cl'},
+      (x \in Γ) ->
+      trans_ Γ e e' ->
+      trans_ Γ (A0.Ecase x cl) (A1.Ecase x w0 cl') ->
+      trans_ Γ (A0.Ecase x ((t, e) :: cl)) (A1.Ecase x w0 ((t, e') :: cl')).
 
-    | Trans_app_unknown :
-      forall {f xs},
-        K ! f = None ->
-        Disjoint _ (FromList xs) (Dom_map K) ->
+  Hint Constructors trans_ : core.
 
-        (f \in Γ) ->
-        (FromList xs \subset Γ) ->
-        trans_ Γ (A0.Eapp f xs) (A1.Eapp f w0 xs)
+  Definition trans := trans_.
 
-    (* data webs are all exposed *)
+  Hint Unfold trans : core.
 
-    | Trans_constr :
-      forall {x t xs k k'},
-        Disjoint _ (FromList xs) (Dom_map K) ->
+  (* Cross-language Logical Relations *)
+  (* Note these are parameterized by the known_map, `K` *)
+  Definition R' (P : nat -> A0.val -> A1.wval -> Prop) (i : nat) (r1 : A0.res) (r2 : A1.res) :=
+    match r1, r2 with
+    | A0.OOT, A1.OOT => True
+    | A0.Res v1, A1.Res v2 => P i v1 v2
+    | _, _ => False
+    end.
 
-        (FromList xs \subset Γ) ->
-        trans_ (x |: Γ) k k' ->
-        trans_ Γ (A0.Econstr x t xs k) (A1.Econstr x w0 t xs k')
+  Definition E' (P : nat -> A0.val -> A1.wval -> Prop) (ex : bool) (i : nat) (ρ1 : A0.env) (e1 :A0.exp) (ρ2 : A1.env) (e2 : A1.exp) : Prop :=
+    forall j1 r1,
+      j1 <= i ->
+      A0.bstep_fuel ρ1 e1 j1 r1 ->
+      exists j2 r2,
+        A1.bstep_fuel ex ρ2 e2 j2 r2 /\
+        R' P (i - j1) r1 r2.
 
-    | Trans_proj :
-      forall {x y k k' n},
-        K ! y = None ->
+  Fixpoint V (i : nat) (v1 : A0.val) (wv2 : A1.wval) {struct i} : Prop :=
+    wf_val wv2 /\
+    match wv2 with
+    | A1.TAG _ w2 v2 =>
+        match v1, v2 with
+        | A0.Vconstr c1 vs1, A1.Vconstr c2 vs2 =>
+            exposed wv2 /\
+            c1 = c2 /\
+            match i with
+            | 0 => length vs1 = length vs2
+            | S i0 => Forall2 (V i0) vs1 vs2
+            end
 
-        (y \in Γ) ->
-        trans_ (x |: Γ) k k' ->
-        trans_ Γ (A0.Eproj x n y k) (A1.Eproj x w0 n y k')
+        | A0.Vfun f1 ρ1 xs1 e1, A1.Vfun f2 ρ2 xs2 e2 =>
+            f1 = f2 /\
+            length xs1 = length xs2 /\
+            match K ! f1 with
+            | None => (* unknown *)
+                exposed wv2 /\
+                match i with
+                | 0 => True
+                | S i0 =>
+                    forall j vs1 vs2 ρ3 ρ4,
+                      j <= i0 ->
+                      Forall exposed vs2 ->
+                      Forall2 (V (i0 - (i0 - j))) vs1 vs2 ->
+                      set_lists xs1 vs1 (M.set f1 (A0.Vfun f1 ρ1 xs1 e1) ρ1) = Some ρ3 ->
+                      set_lists xs2 vs2 (M.set f2 (Tag w2 (A1.Vfun f2 ρ2 xs2 e2)) ρ2) = Some ρ4 ->
+                      E' V true (i0 - (i0 - j)) ρ3 e1 ρ4 e2
+                end
+            | Some w1 => (* known *)
+                w1 = w2 /\
+                (~ w1 \in Exposed) /\
+                match i with
+                | 0 => True
+                | S i0 =>
+                    forall j vs1 vs2 ρ3 ρ4,
+                      j <= i0 ->
+                      Forall2 (V (i0 - (i0 - j))) vs1 vs2 ->
+                      set_lists xs1 vs1 (M.set f1 (A0.Vfun f1 ρ1 xs1 e1) ρ1) = Some ρ3 ->
+                      set_lists xs2 vs2 (M.set f2 (Tag w2 (A1.Vfun f2 ρ2 xs2 e2)) ρ2) = Some ρ4 ->
+                      E' V false (i0 - (i0 - j)) ρ3 e1 ρ4 e2
+                end
+            end
+        | _, _ => False
+        end
+    end.
 
-    | Trans_case_nil :
-      forall {x},
-        (x \in Γ) ->
-        trans_ Γ (A0.Ecase x []) (A1.Ecase x w0 [])
+  Definition R := (R' V).
 
-    | Trans_case_cons :
-      forall {x e e' t cl cl'},
-        (x \in Γ) ->
-        trans_ Γ e e' ->
-        trans_ Γ (A0.Ecase x cl) (A1.Ecase x w0 cl') ->
-        trans_ Γ (A0.Ecase x ((t, e) :: cl)) (A1.Ecase x w0 ((t, e') :: cl')).
+  Definition E := (E' V).
 
-    Hint Constructors trans_ : core.
+  Lemma trans_exp_inv {Γ e e'} :
+    trans Γ e e' ->
+    (A1.occurs_free e') \subset (A0.occurs_free e).
+  Proof.
+    unfold Ensembles.Included, Ensembles.In.
+    intros H.
+    induction H; simpl; intros; auto.
+    - inv H1; auto.
+    - inv H3; auto.
+    - inv H2; auto.
+    - inv H4; auto.
+    - inv H3; auto.
+    - inv H2; auto.
+    - inv H2; auto.
+    - inv H0; auto.
+    - inv H2; auto.
+  Qed.
 
-    Definition trans := trans_.
+  Lemma trans_exp_weaken {Γ Γ' e e'} :
+    trans Γ e e' ->
+    Γ \subset Γ' ->
+    trans Γ' e e'.
+  Proof.
+  Admitted.
 
-    Hint Unfold trans : core.
+  Theorem trans_total :
+    forall e,
+    exists e',
+      trans (A0.occurs_free e) e e'.
+  Proof.
+  Admitted.
 
-    (* Cross-language Logical Relations *)
-    (* Note this is parameterized by known_map, `K` *)
-    Definition R' (P : nat -> A0.val -> A1.wval -> Prop) (i : nat) (r1 : A0.res) (r2 : A1.res) :=
-      match r1, r2 with
-      | A0.OOT, A1.OOT => True
-      | A0.Res v1, A1.Res v2 => P i v1 v2
-      | _, _ => False
-      end.
+  Lemma Erase_Annotate_id e1 e2 e1' :
+    trans (A0.occurs_free e1) e1 e1' ->
+    Erase.trans (A1.occurs_free e1') e1' e2 ->
+    e1 = e2.
+  Proof.
+  Admitted.
 
-    Definition E' (P : nat -> A0.val -> A1.wval -> Prop) (ex : bool) (i : nat) (ρ1 : A0.env) (e1 :A0.exp) (ρ2 : A1.env) (e2 : A1.exp) : Prop :=
-      forall j1 r1,
-        j1 <= i ->
-        A0.bstep_fuel ρ1 e1 j1 r1 ->
-        exists j2 r2,
-          A1.bstep_fuel ex ρ2 e2 j2 r2 /\
-          R' P (i - j1) r1 r2.
+  (* Lemmas about [wf_val], [wf_res], and [wf_env] *)
+  Lemma V_wf_val_r {i v1 v2}:
+    V i v1 v2 ->
+    wf_val v2.
+  Proof.
+    intros HV.
+    destruct i; simpl in *;
+      destruct HV as [Hv2 _]; auto.
+  Qed.
 
-    Fixpoint V (i : nat) (v1 : A0.val) (wv2 : A1.wval) {struct i} : Prop :=
-      wf_val wv2 /\
-      match wv2 with
-      | A1.TAG _ w2 v2 =>
-          match v1, v2 with
-          | A0.Vconstr c1 vs1, A1.Vconstr c2 vs2 =>
-              exposed wv2 /\
-              c1 = c2 /\
-              match i with
-              | 0 => length vs1 = length vs2
-              | S i0 => Forall2 (V i0) vs1 vs2
-              end
+  Lemma V_wf_val_Forall_r {i vs1 vs2} :
+    Forall2 (V i) vs1 vs2 ->
+    Forall wf_val vs2.
+  Proof.
+    intros.
+    induction H; auto.
+    constructor; auto.
+    eapply V_wf_val_r; eauto.
+  Qed.
 
-          | A0.Vfun f1 ρ1 xs1 e1, A1.Vfun f2 ρ2 xs2 e2 =>
-              length xs1 = length xs2 /\
-              match K ! f1 with
-              | None => (* unknown *)
-                  exposed wv2 /\
-                  match i with
-                  | 0 => True
-                  | S i0 =>
-                      forall j vs1 vs2 ρ3 ρ4,
-                        j <= i0 ->
-                        Forall exposed vs2 ->
-                        Forall2 (V (i0 - (i0 - j))) vs1 vs2 ->
-                        set_lists xs1 vs1 (M.set f1 (A0.Vfun f1 ρ1 xs1 e1) ρ1) = Some ρ3 ->
-                        set_lists xs2 vs2 (M.set f2 (Tag w2 (A1.Vfun f2 ρ2 xs2 e2)) ρ2) = Some ρ4 ->
-                        E' V true (i0 - (i0 - j)) ρ3 e1 ρ4 e2
-                  end
-              | Some w1 => (* known *)
-                  w1 = w2 /\
-                  (~ w1 \in Exposed) /\
-                  match i with
-                  | 0 => True
-                  | S i0 =>
-                      forall j vs1 vs2 ρ3 ρ4,
-                        j <= i0 ->
-                        Forall2 (V (i0 - (i0 - j))) vs1 vs2 ->
-                        set_lists xs1 vs1 (M.set f1 (A0.Vfun f1 ρ1 xs1 e1) ρ1) = Some ρ3 ->
-                        set_lists xs2 vs2 (M.set f2 (Tag w2 (A1.Vfun f2 ρ2 xs2 e2)) ρ2) = Some ρ4 ->
-                        E' V false (i0 - (i0 - j)) ρ3 e1 ρ4 e2
-                  end
-              end
-          | _, _ => False
-          end
-      end.
+  Lemma V_wf_res_r {i v1 v2}:
+    V i v1 v2 ->
+    wf_res (Res v2).
+  Proof.
+    intros HV.
+    constructor.
+    eapply V_wf_val_r; eauto.
+  Qed.
 
-    Definition R := (R' V).
+  Lemma R_wf_res_l {i r1 r2} :
+    R i r1 r2 ->
+    wf_res r2.
+  Proof.
+    unfold R.
+    intros.
+    destruct r1; destruct r2; try contradiction; auto.
+    constructor.
+    eapply V_wf_val_r; eauto.
+  Qed.
 
-    Definition E := (E' V).
+  (* Inversion Lemmas *)
+  Lemma R_res_inv_l i v1 r2 :
+    R i (A0.Res v1) r2 ->
+    exists v2, r2 = A1.Res v2 /\ V i v1 v2.
+  Proof.
+    intros.
+    destruct r2; simpl in *; try contradiction.
+    eexists; split; eauto.
+  Qed.
 
-    Lemma trans_exp_inv {Γ e e'} :
-      trans Γ e e' ->
-      (A1.occurs_free e') \subset (A0.occurs_free e).
-    Proof.
-      unfold Ensembles.Included, Ensembles.In.
-      intros H.
-      induction H; simpl; intros; auto.
-      - inv H1; auto.
-      - inv H3; auto.
-      - inv H2; auto.
-      - inv H4; auto.
-      - inv H3; auto.
-      - inv H2; auto.
-      - inv H2; auto.
-      - inv H0; auto.
-      - inv H2; auto.
-    Qed.
+  (* Environment Relation *)
+  Definition same_id x wv2 :=
+    match wv2 with
+    | A1.TAG _ w2 v2 =>
+        match v2 with
+        | A1.Vfun f2 ρ2 xs2 e2 => f2 = x
+        | A1.Vconstr c2 vs2 => True
+        end
+    end.
 
-    Lemma trans_exp_weaken {Γ Γ' e e'} :
-      trans Γ e e' ->
-      Γ \subset Γ' ->
-      trans Γ' e e'.
-    Proof.
-    Admitted.
+  Lemma same_id_fun f w f1 t l e:
+    same_id f (TAG val w (Vfun f1 t l e)) -> f1 = f.
+  Proof. unfold same_id; simpl; auto. Qed.
 
-    Theorem trans_complete :
-      forall e,
-        exists e',
-          trans (A0.occurs_free e) e e'.
-    Proof.
-    Admitted.
-
-    Lemma Erase_Annotate_id e1 e2 e1' :
-      trans (A0.occurs_free e1) e1 e1' ->
-      Erase.trans (A1.occurs_free e1') e1' e2 ->
-      e1 = e2.
-    Proof.
-    Admitted.
-
-    (* Lemmas about [wf_val], [wf_res], and [wf_env] *)
-    Lemma V_wf_val_r {i v1 v2}:
-      V i v1 v2 ->
-      wf_val v2.
-    Proof.
-      intros HV.
-      destruct i; simpl in *;
-        destruct HV as [Hv2 _]; auto.
-    Qed.
-
-    Lemma V_wf_val_Forall_r {i vs1 vs2} :
-      Forall2 (V i) vs1 vs2 ->
-      Forall wf_val vs2.
-    Proof.
-      intros.
-      induction H; auto.
-      constructor; auto.
-      eapply V_wf_val_r; eauto.
-    Qed.
-
-    Lemma V_wf_res_r {i v1 v2}:
-      V i v1 v2 ->
-      wf_res (Res v2).
-    Proof.
-      intros HV.
-      constructor.
-      eapply V_wf_val_r; eauto.
-    Qed.
-
-    Lemma R_wf_res_l {i r1 r2} :
-      R i r1 r2 ->
-      wf_res r2.
-    Proof.
-      unfold R.
-      intros.
-      destruct r1; destruct r2; try contradiction; auto.
-      constructor.
-      eapply V_wf_val_r; eauto.
-    Qed.
-
-    (* Inversion Lemmas *)
-    Lemma R_res_inv_l i v1 r2 :
-      R i (A0.Res v1) r2 ->
-      exists v2, r2 = A1.Res v2 /\ V i v1 v2.
-    Proof.
-      intros.
-      destruct r2; simpl in *; try contradiction.
-      eexists; split; eauto.
-    Qed.
-
-    (* Environment Relation *)
-    Definition G i Γ1 ρ1 Γ2 ρ2 :=
-      wf_env ρ2 /\
-      forall x,
-        (x \in Γ1) ->
-        forall v1,
-          M.get x ρ1 = Some v1 ->
-          ((x \in Γ2) ->
-          exists v2,
-            M.get x ρ2 = Some v2 /\
-            V i v1 v2).
-
-    Definition trans_correct Γ e1 e2 :=
-      forall ex i ρ1 ρ2,
-        G i Γ ρ1 (A1.occurs_free e2) ρ2 ->
-        E ex i ρ1 e1 ρ2 e2.
-
-    (* Environment Lemmas *)
-    Lemma G_wf_env_r {i Γ1 ρ1 Γ2 ρ2}:
-      G i Γ1 ρ1 Γ2 ρ2 ->
-      wf_env ρ2.
-    Proof.
-      unfold G.
-      intros H; destruct H; auto.
-    Qed.
-
-    Lemma G_get {Γ1 Γ2 i ρ1 ρ2}:
-      G i Γ1 ρ1 Γ2 ρ2 ->
-      forall x v1,
-        (x \in Γ1) ->
-        (x \in Γ2) ->
+  (* TODO: refactor *)
+  Definition G i Γ1 ρ1 Γ2 ρ2 :=
+    wf_env ρ2 /\
+    forall x,
+      (x \in Γ1) ->
+      forall v1,
         M.get x ρ1 = Some v1 ->
-        exists v2,
-          M.get x ρ2 = Some v2 /\
-          V i v1 v2.
-    Proof.
-      unfold G.
-      intros.
-      destruct H as [Hr1 HG].
-      eapply HG; eauto.
-    Qed.
+        ((x \in Γ2) ->
+         exists v2,
+           M.get x ρ2 = Some v2 /\
+           same_id x v2 /\
+           (K ! x = None -> exposed v2) /\
+           V i v1 v2).
 
-    Lemma G_get_list {i Γ1 ρ1 Γ2 ρ2} :
-      G i Γ1 ρ1 Γ2 ρ2 ->
-      forall xs vs1,
-        (FromList xs) \subset Γ1 ->
-        (FromList xs) \subset Γ2 ->
-        get_list xs ρ1 = Some vs1 ->
-        exists vs2,
-          get_list xs ρ2 = Some vs2 /\
-          Forall2 (V i) vs1 vs2.
-    Proof.
-      unfold G.
-      intros HG xs.
-      induction xs; simpl; intros.
-      - inv H1; eauto.
-      - destruct (ρ1 ! a) eqn:Heq1; try discriminate.
-        destruct (get_list xs ρ1) eqn:Heq3; try discriminate.
-        inv H1.
-        unfold Ensembles.Included, Ensembles.In, FromList in *.
-        edestruct (G_get HG) as [v2 [Heqv2 HV]]; eauto.
-        eapply (H a).
-        apply in_eq.
+  (* Environment Lemmas *)
+  Lemma G_wf_env_r {i Γ1 ρ1 Γ2 ρ2}:
+    G i Γ1 ρ1 Γ2 ρ2 ->
+    wf_env ρ2.
+  Proof.
+    unfold G.
+    intros H; destruct H; auto.
+  Qed.
+
+  Lemma G_get {Γ1 Γ2 i ρ1 ρ2}:
+    G i Γ1 ρ1 Γ2 ρ2 ->
+    forall x v1,
+      (x \in Γ1) ->
+      (x \in Γ2) ->
+      M.get x ρ1 = Some v1 ->
+      exists v2,
+        M.get x ρ2 = Some v2 /\
+        same_id x v2 /\
+        (K ! x = None -> exposed v2) /\
+        V i v1 v2.
+  Proof.
+    unfold G.
+    intros.
+    destruct H as [Hr1 HG].
+    eapply HG; eauto.
+  Qed.
+
+  Lemma G_get_list {i Γ1 ρ1 Γ2 ρ2} :
+    G i Γ1 ρ1 Γ2 ρ2 ->
+    forall xs vs1,
+      (FromList xs) \subset Γ1 ->
+      (FromList xs) \subset Γ2 ->
+      Disjoint _ (FromList xs) (Dom_map K) ->
+      get_list xs ρ1 = Some vs1 ->
+      exists vs2,
+        get_list xs ρ2 = Some vs2 /\
+        Forall exposed vs2 /\
+        Forall2 (V i) vs1 vs2.
+  Proof.
+    intros HG xs.
+    induction xs; simpl; intros.
+    - inv H2; eauto.
+    - destruct (ρ1 ! a) eqn:Heq1; try discriminate.
+      destruct (get_list xs ρ1) eqn:Heq3; try discriminate.
+      inv H2.
+      unfold Ensembles.Included, Ensembles.In in *.
+      edestruct (G_get HG) as [v2 [Heqv2 [Hid [HK HV]]]]; eauto.
+      eapply (H a).
+      apply in_eq.
+      apply H0.
+      apply in_eq.
+      edestruct IHxs as [vs2 [Heqvs2 [Hexvs2 Vvs]]]; eauto.
+      + intros.
+        apply H.
+        apply in_cons; auto.
+      + intros.
         apply H0.
-        apply in_eq.
-        edestruct IHxs as [vs2 [Heqvs2 Vvs]]; eauto.
-        + intros.
-          apply H.
-          apply in_cons; auto.
-        + intros.
-          apply H0.
-          apply in_cons; auto.
-        + rewrite Heqvs2.
-          exists (v2 :: vs2); split; auto.
-          rewrite Heqv2; auto.
-    Qed.
+        apply in_cons; auto.
+      + eapply Disjoint_FromList_cons_l; eauto.
+      + rewrite Heqvs2.
+        exists (v2 :: vs2); split; auto.
+        rewrite Heqv2; auto.
+        split; auto.
+        constructor; auto.
+        apply Disjoint_FromList_cons_inv in H1.
+        inv H1.
+        apply not_Dom_map_eq in H2; auto.
+  Qed.
 
-    Lemma G_set {i Γ1 ρ1 Γ2 ρ2}:
-      G i Γ1 ρ1 Γ2 ρ2 ->
-      forall {x v1 v2},
-        V i v1 v2 ->
-        G i (x |: Γ1) (M.set x v1 ρ1) (x |: Γ2) (M.set x v2 ρ2).
-    Proof.
-      unfold G.
-      intros.
+  (*
+  Lemma G_set {i Γ1 ρ1 Γ2 ρ2}:
+    G i Γ1 ρ1 Γ2 ρ2 ->
+    forall {x v1 v2},
+      V i v1 v2 ->
+      G i (x |: Γ1) (M.set x v1 ρ1) (x |: Γ2) (M.set x v2 ρ2).
+  Proof.
+    unfold G.
+    intros.
 
+    inv H.
+    split.
+    eapply wf_env_set; eauto.
+    eapply V_wf_val_r; eauto.
+
+    intros.
+    destruct (M.elt_eq x0 x); subst.
+    - repeat rewrite M.gss in *.
+      inv H3.
+      eexists; split; eauto; intros.
+    - rewrite M.gso in *; auto.
       inv H.
+      inv H5; try contradiction.
+      inv H4.
+      inv H; try contradiction.
+      edestruct H2 as [v1' [Heqv1' Hv2]]; eauto.
+  Qed.
+
+  Lemma G_set_lists {i Γ1 ρ1 Γ2 ρ2}:
+    G i Γ1 ρ1 Γ2 ρ2 ->
+    forall {xs vs1 vs2 ρ3 ρ4},
+      Forall2 (V i) vs1 vs2 ->
+      set_lists xs vs1 ρ1 = Some ρ3 ->
+      set_lists xs vs2 ρ2 = Some ρ4 ->
+      G i (FromList xs :|: Γ1) ρ3 (FromList xs :|: Γ2) ρ4.
+  Proof.
+    intros HG xs.
+    induction xs; simpl; intros.
+    - destruct vs1; try discriminate.
+      destruct vs2; try discriminate.
+      inv H0; inv H1.
+      unfold G.
+      split; intros.
+      eapply G_wf_env_r; eauto.
+
+      eapply (G_get HG); eauto.
+      inv H0; auto.
+      inv H3.
+
+      inv H2; auto.
+      inv H3.
+    - destruct vs1; try discriminate.
+      destruct vs2; try discriminate.
+      destruct (set_lists xs vs1 ρ1) eqn:Heq1; try discriminate.
+      destruct (set_lists xs vs2 ρ2) eqn:Heq2; try discriminate.
+      inv H; inv H0; inv H1.
+      unfold G.
+
       split.
       eapply wf_env_set; eauto.
+      eapply (wf_env_set_lists ρ2) with (xs := xs) (vs := vs2); eauto.
+
+      eapply G_wf_env_r; eauto.
+      eapply V_wf_val_Forall_r; eauto.
       eapply V_wf_val_r; eauto.
 
       intros.
-      destruct (M.elt_eq x0 x); subst.
-      - repeat rewrite M.gss in *.
-        inv H3.
-        eexists; split; eauto; intros.
-      - rewrite M.gso in *; auto.
-        inv H.
-        inv H5; try contradiction.
-        inv H4.
-        inv H; try contradiction.
-        edestruct H2 as [v1' [Heqv1' Hv2]]; eauto.
-    Qed.
+      destruct (M.elt_eq x a); subst.
+      + repeat rewrite M.gss in *; eauto.
+        inv H0.
+        eexists; split; eauto.
+      + rewrite M.gso in *; auto.
+        eapply IHxs; eauto.
+        eapply not_In_cons_Union; eauto.
+        eapply not_In_cons_Union; eauto.
+  Qed.
+*)
+  Lemma G_subset Γ1 Γ2 {i ρ1 Γ3 ρ2 Γ4}:
+    G i Γ1 ρ1 Γ2 ρ2 ->
+    Γ3 \subset Γ1 ->
+    Γ4 \subset Γ2 ->
+    G i Γ3 ρ1 Γ4 ρ2.
+  Proof.
+    unfold G.
+    intros.
+    inv H; split; auto.
+  Qed.
 
-    Lemma G_set_lists {i Γ1 ρ1 Γ2 ρ2}:
-      G i Γ1 ρ1 Γ2 ρ2 ->
-      forall {xs vs1 vs2 ρ3 ρ4},
-        Forall2 (V i) vs1 vs2 ->
-        set_lists xs vs1 ρ1 = Some ρ3 ->
-        set_lists xs vs2 ρ2 = Some ρ4 ->
-        G i (FromList xs :|: Γ1) ρ3 (FromList xs :|: Γ2) ρ4.
-    Proof.
-      intros HG xs.
-      induction xs; simpl; intros.
-      - destruct vs1; try discriminate.
-        destruct vs2; try discriminate.
-        inv H0; inv H1.
-        unfold G.
-        split; intros.
-        eapply G_wf_env_r; eauto.
-
-        eapply (G_get HG); eauto.
-        inv H0; auto.
-        inv H3.
-
-        inv H2; auto.
-        inv H3.
-      - destruct vs1; try discriminate.
-        destruct vs2; try discriminate.
-        destruct (set_lists xs vs1 ρ1) eqn:Heq1; try discriminate.
-        destruct (set_lists xs vs2 ρ2) eqn:Heq2; try discriminate.
-        inv H; inv H0; inv H1.
-        unfold G.
-
-        split.
-        eapply wf_env_set; eauto.
-        eapply (wf_env_set_lists ρ2) with (xs := xs) (vs := vs2); eauto.
-
-        eapply G_wf_env_r; eauto.
-        eapply V_wf_val_Forall_r; eauto.
-        eapply V_wf_val_r; eauto.
-
-        intros.
-        destruct (M.elt_eq x a); subst.
-        + repeat rewrite M.gss in *; eauto.
-          inv H0.
-          eexists; split; eauto.
-        + rewrite M.gso in *; auto.
-          eapply IHxs; eauto.
-          eapply not_In_cons_Union; eauto.
-          eapply not_In_cons_Union; eauto.
-    Qed.
-
-    Lemma G_subset Γ1 Γ2 {i ρ1 Γ3 ρ2 Γ4}:
-      G i Γ1 ρ1 Γ2 ρ2 ->
-      Γ3 \subset Γ1 ->
-      Γ4 \subset Γ2 ->
-      G i Γ3 ρ1 Γ4 ρ2.
-    Proof.
-      unfold G.
-      intros.
-      inv H; split; auto.
-    Qed.
-
-    (* Monotonicity Lemmas *)
-    Lemma V_mono_Forall_aux :
-      forall i j (V : nat -> A0.val -> A1.wval -> Prop) vs1 vs2,
-        (forall k : nat,
-            k < S i ->
-            forall (j : nat) v1 v2, V k v1 v2 -> j <= k -> V j v1 v2) ->
-        Forall2 (V i) vs1 vs2 ->
-        j <= i ->
-        Forall2 (V j) vs1 vs2.
-    Proof.
-      intros.
-      revert vs2 H0.
-      induction vs1; intros; inv H0; auto.
-      rename l' into vs2.
-      constructor; auto.
-      eapply H; eauto; lia.
-    Qed.
-
-    Lemma V_mono i :
-      forall {j v1 v2},
-        V i v1 v2 ->
-        j <= i ->
-        V j v1 v2.
-    Proof.
-      induction i using lt_wf_rec; intros.
-      destruct v2.
-      destruct i; simpl in H0;
-        destruct j; simpl; intros;
-        destruct H0 as [Hv1 HV]; subst.
-      - repeat (split; auto).
-      - inv H1.
-      - repeat (split; auto).
-        destruct v1; destruct v; try contradiction.
-        + destruct HV.
-          destruct (K ! v0) eqn:HeqK.
-          * destruct H2 as [Heqw [Hex HV]]; subst.
-            repeat (split; eauto).
-          * destruct H2 as [Hex HV].
-            repeat (split; eauto).
-        + destruct HV as [Hex [Hc HV]]; subst.
-          repeat split; auto.
-          eapply Forall2_length; eauto.
-      - repeat (split; auto).
-        destruct v1; destruct v; try contradiction;
-          destruct HV as [Hlen HV]; subst.
-        + destruct (K ! v0) eqn:HeqK.
-          * destruct HV as [Heqw [Hex HV]]; subst.
-            repeat (split; eauto); intros.
-            specialize (HV j0 vs1 vs2 ρ3 ρ4).
-            rewrite normalize_step in *; try lia.
-            apply HV; eauto; lia.
-          * destruct HV as [Hex HV]; subst.
-            repeat split; auto; intros.
-            specialize (HV j0 vs1 vs2 ρ3 ρ4).
-            rewrite normalize_step in *; try lia.
-            eapply HV; eauto; lia.
-        + destruct HV as [Heqc HV]; subst.
-          repeat split; auto.
-          eapply V_mono_Forall_aux; eauto; lia.
-    Qed.
-
-    Lemma V_mono_Forall {vs1 vs2} i j :
+  (* Monotonicity Lemmas *)
+  Lemma V_mono_Forall_aux :
+    forall i j (V : nat -> A0.val -> A1.wval -> Prop) vs1 vs2,
+      (forall k : nat,
+          k < S i ->
+          forall (j : nat) v1 v2, V k v1 v2 -> j <= k -> V j v1 v2) ->
       Forall2 (V i) vs1 vs2 ->
       j <= i ->
       Forall2 (V j) vs1 vs2.
-    Proof.
-      intros H.
-      revert j.
-      induction H; simpl; intros; auto.
-      constructor; eauto.
-      eapply V_mono; eauto.
-    Qed.
+  Proof.
+    intros.
+    revert vs2 H0.
+    induction vs1; intros; inv H0; auto.
+    rename l' into vs2.
+    constructor; auto.
+    eapply H; eauto; lia.
+  Qed.
 
-    Lemma R_mono {r1 r2} i j :
-      R i r1 r2 ->
+  Lemma V_mono i :
+    forall {j v1 v2},
+      V i v1 v2 ->
       j <= i ->
-      R j r1 r2.
-    Proof.
-      unfold R.
-      intros.
-      destruct r1; auto.
-      destruct r2; auto.
-      eapply V_mono; eauto.
-    Qed.
+      V j v1 v2.
+  Proof.
+    induction i using lt_wf_rec; intros.
+    destruct v2.
+    destruct i; simpl in H0;
+      destruct j; simpl; intros;
+      destruct H0 as [Hv1 HV]; subst.
+    - repeat (split; auto).
+    - inv H1.
+    - repeat (split; auto).
+      destruct v1; destruct v; try contradiction.
+      + destruct HV.
+        destruct (K ! v0) eqn:HeqK.
+        * destruct H2 as [Hlen [Heqw [Hex HV]]]; subst.
+          repeat (split; eauto).
+        * destruct H2 as [Hlen [Hex HV]].
+          repeat (split; eauto).
+      + destruct HV as [Hex [Hc HV]]; subst.
+        repeat split; auto.
+        eapply Forall2_length; eauto.
+    - repeat (split; auto).
+      destruct v1; destruct v; try contradiction.
+      + destruct HV as [Hf [Hlen HV]]; subst.
+        repeat split; auto.
+        destruct (K ! v) eqn:HeqK.
+        * destruct HV as [Heqw [Hex HV]]; subst.
+          repeat split; auto; intros.
+          specialize (HV j0 vs1 vs2 ρ3 ρ4).
+          rewrite normalize_step in *; try lia.
+          apply HV; eauto; lia.
+        * destruct HV as [Hex HV]; subst.
+          repeat split; auto; intros.
+          specialize (HV j0 vs1 vs2 ρ3 ρ4).
+          rewrite normalize_step in *; try lia.
+          eapply HV; eauto; lia.
+      + destruct HV as [Hex [Heqc HV]]; subst.
+        repeat split; auto.
+        eapply V_mono_Forall_aux; eauto; lia.
+  Qed.
 
-    Lemma E_mono {ex ρ1 ρ2 e1 e2} i j:
-      E ex i ρ1 e1 ρ2 e2 ->
-      j <= i ->
-      E ex j ρ1 e1 ρ2 e2.
-    Proof.
-      unfold E, R, E', R'.
-      intros.
-      destruct (H j1 r1) as [j2 [r2 [Hr2 HR]]]; auto; try lia.
-      exists j2, r2; split; eauto.
-      apply R_mono with (i - j1); try lia; auto.
-    Qed.
+  Lemma V_mono_Forall {vs1 vs2} i j :
+    Forall2 (V i) vs1 vs2 ->
+    j <= i ->
+    Forall2 (V j) vs1 vs2.
+  Proof.
+    intros H.
+    revert j.
+    induction H; simpl; intros; auto.
+    constructor; eauto.
+    eapply V_mono; eauto.
+  Qed.
 
-    Lemma G_mono {Γ1 Γ2 ρ1 ρ2} i j:
-      G i Γ1 ρ1 Γ2 ρ2 ->
-      j <= i ->
-      G j Γ1 ρ1 Γ2 ρ2.
-    Proof.
-      unfold G.
-      intros.
-      inv H.
-      split; auto; intros.
-      edestruct H2 as [v2 [Heqv2 HV]]; eauto.
-      eexists; eexists; repeat split; eauto.
-      apply V_mono with i; eauto.
-    Qed.
+  Lemma R_mono {r1 r2} i j :
+    R i r1 r2 ->
+    j <= i ->
+    R j r1 r2.
+  Proof.
+    unfold R.
+    intros.
+    destruct r1; auto.
+    destruct r2; auto.
+    eapply V_mono; eauto.
+  Qed.
 
-    (* Fundamental Property *)
-    Lemma fundamental_property {Γ e e'}:
-      trans Γ e e' -> trans_correct Γ e e'.
-    Proof.
-      intros H.
-      induction H.
-      - admit.
-      - admit.
-      - admit.
-      - admit.
-      - admit.
-      - admit.
-      - admit.
-      - admit.
-    Admitted.
+  Lemma E_mono {ex ρ1 ρ2 e1 e2} i j:
+    E ex i ρ1 e1 ρ2 e2 ->
+    j <= i ->
+    E ex j ρ1 e1 ρ2 e2.
+  Proof.
+    unfold E, R, E', R'.
+    intros.
+    destruct (H j1 r1) as [j2 [r2 [Hr2 HR]]]; auto; try lia.
+    exists j2, r2; split; eauto.
+    apply R_mono with (i - j1); try lia; auto.
+  Qed.
 
-    (* Top Level *)
-    Definition G_top i Γ1 ρ1 Γ2 ρ2 :=
-      wf_env ρ2 /\
+  Lemma G_mono {Γ1 Γ2 ρ1 ρ2} i j:
+    G i Γ1 ρ1 Γ2 ρ2 ->
+    j <= i ->
+    G j Γ1 ρ1 Γ2 ρ2.
+  Proof.
+    unfold G.
+    intros.
+    inv H.
+    split; auto; intros.
+    edestruct H2 as [v2 [Heqv2 [Hid [HK HV]]]]; eauto.
+    eexists; eexists; repeat split; eauto.
+    apply V_mono with i; eauto.
+  Qed.
+
+  (* Compatibility Lemmas *)
+  Definition unknownb (e : A1.exp) :=
+    match e with
+    | A1.Efun f w xs e k => exposedb w
+    | A1.Eapp f w xs => exposedb w
+    | A1.Eletapp x f w xs k => exposedb w
+    | _ => true
+    end.
+
+  Definition trans_correct Γ e1 e2 :=
+    forall i ρ1 ρ2,
+      known_map_inv K ->
+      G i Γ ρ1 (A1.occurs_free e2) ρ2 ->
+      E (unknownb e2) i ρ1 e1 ρ2 e2.
+
+  Lemma ret_compat Γ x :
+    (x \in Γ) ->
+    K ! x = None ->
+    trans_correct Γ (A0.Eret x) (A1.Eret x).
+  Proof.
+    unfold trans_correct, E, E', R, R', Ensembles.Included, Ensembles.In, Dom_map.
+    intros; simpl.
+    inv H4.
+    - exists 0, A1.OOT; split; auto.
+    - inv H5.
+      edestruct (G_get H2) as [v2 [Heqv2 [Hid [HK HV]]]]; eauto.
+      exists 1, (A1.Res v2); split; auto.
+      apply V_mono with i; try lia; auto.
+  Qed.
+
+  Lemma app_known_compat Γ xs f w :
+    (K ! f = Some w) ->
+    (~ w \in Exposed) ->
+    Disjoint _ (FromList xs) (Dom_map K) ->
+
+    (f \in Γ) ->
+    (FromList xs \subset Γ) ->
+    trans_correct Γ (A0.Eapp f xs) (A1.Eapp f w xs).
+  Proof.
+    unfold trans_correct, E, E'.
+    intros HKf Hw HKxs.
+    intros; simpl.
+
+    inv H4.
+    - exists 0, A1.OOT; split; simpl; auto.
+    - inv H5.
+      edestruct (G_get H2 f) as [fv2 [Heqfv2 [Hid [HK HV]]]]; eauto.
+      destruct i.
+      inv H3.
+      destruct fv2; simpl in HV;
+        destruct HV as [Hv1 HV];
+        destruct v; try contradiction.
+      apply same_id_fun in Hid; inv Hid.
+      destruct HV as [Hfeq [Hlen HV]]; subst.
+      destruct (K ! f) eqn:Heqk; try contradiction.
+      + destruct HV as [Heqw [Hex HV]]; subst.
+        inv HKf.
+        clear HK Hex.
+
+        edestruct (G_get_list H2 xs vs) as [vs2 [Heqvs2 [Hexvs Vvs]]]; eauto.
+        eapply A1.free_app_xs_subset; eauto.
+
+        destruct (set_lists_length3 (M.set f (Tag w (A1.Vfun f t l e0)) t) l vs2) as [ρ4 Heqρ4].
+        unfold wval in *.
+        rewrite <- (Forall2_length _ _ _ Vvs).
+        rewrite <- (set_lists_length_eq _ _ _ _ H9); auto.
+
+        assert (HE : E false (i - (i - i)) ρ'' e ρ4 e0).
+        {
+          eapply (HV i vs vs2); eauto.
+          apply V_mono_Forall with (S i); auto; lia.
+        }
+
+        apply (E_mono _ i) in HE; try lia.
+        unfold E in HE.
+        destruct (HE c r1) as [j2 [r2 [He0 Rr]]]; try lia; auto.
+        exists (S j2), r2; split; eauto.
+        constructor; auto.
+        * econstructor; eauto.
+          destruct (exposed_reflect w); try contradiction; auto.
+          intros; contradiction.
+        * destruct (exposed_reflect w); try contradiction; auto.
+      + destruct HV as [Hex HV].
+        inv Hex.
+        rewrite HKf in Heqk; discriminate.
+  Qed.
+
+  Lemma app_unknown_compat Γ xs f :
+    (K ! f = None) ->
+    Disjoint _ (FromList xs) (Dom_map K) ->
+
+    (f \in Γ) ->
+    (FromList xs \subset Γ) ->
+    trans_correct Γ (A0.Eapp f xs) (A1.Eapp f w0 xs).
+  Proof.
+    unfold trans_correct, E, E'.
+    intros HKf HKxs.
+    intros.
+    inv H4.
+    - exists 0, A1.OOT; split; simpl; auto.
+    - inv H5.
+      edestruct (G_get H2 f) as [fv2 [Heqfv2 [Hid [HK HV]]]]; eauto.
+      destruct i.
+      inv H3.
+      destruct fv2; simpl in HV;
+        destruct HV as [Hv1 HV];
+        destruct v; try contradiction.
+      apply same_id_fun in Hid; inv Hid.
+      destruct HV as [Hfeq [Hlen HV]]; subst.
+      destruct (K ! f) eqn:Heqk; try discriminate.
+      destruct HV as [Hex HV].
+      inv Hex.
+      assert (Hw : w = w0) by (apply Exposed_singleton; eauto); subst.
+
+      edestruct (G_get_list H2 xs vs) as [vs2 [Heqvs2 [Hexvs Vvs]]]; eauto.
+      eapply A1.free_app_xs_subset; eauto.
+
+      destruct (set_lists_length3 (M.set f (Tag w0 (A1.Vfun f t l e0)) t) l vs2) as [ρ4 Heqρ4].
+      unfold wval in *.
+      rewrite <- (Forall2_length _ _ _ Vvs).
+      rewrite <- (set_lists_length_eq _ _ _ _ H9); auto.
+
+      assert (HE : E true (i - (i - i)) ρ'' e ρ4 e0).
+      {
+        eapply (HV i vs vs2); eauto.
+        apply V_mono_Forall with (S i); auto; lia.
+      }
+
+      apply (E_mono _ i) in HE; try lia.
+      unfold E in HE.
+      destruct (HE c r1) as [j2 [r2 [He0 Rr]]]; try lia; auto.
+      assert (exposed_res r2) by (eapply bstep_fuel_exposed_inv; eauto).
+      exists (S j2), r2; split; eauto; simpl.
+      constructor; auto.
+      * econstructor; eauto.
+        destruct (exposed_reflect w0); try contradiction; auto.
+      * destruct (exposed_reflect w0); try contradiction; auto.
+  Qed.
+
+  (* Fundamental Property *)
+  Lemma fundamental_property {Γ e e'}:
+    trans Γ e e' -> trans_correct Γ e e'.
+  Proof.
+    intros H.
+    induction H.
+    - eapply ret_compat; eauto.
+    - admit.
+    - admit.
+    - eapply app_known_compat; eauto.
+    - eapply app_unknown_compat; eauto.
+    - admit.
+    - admit.
+    - admit.
+  Admitted.
+
+  (* Top Level *)
+  Definition G_top i Γ1 ρ1 Γ2 ρ2 :=
+    wf_env ρ2 /\
       Γ2 \subset Γ1 /\
       forall x,
         (x \in Γ1) ->
         exists v1 v2,
           M.get x ρ1 = Some v1 /\
-          M.get x ρ2 = Some v2 /\
-          exposed v2 /\
-          V i v1 v2.
+            M.get x ρ2 = Some v2 /\
+            exposed v2 /\
+            V i v1 v2.
 
-    Lemma G_top_wf_env_r i Γ1 ρ1 Γ2 ρ2 :
+  Lemma G_top_wf_env_r i Γ1 ρ1 Γ2 ρ2 :
+    G_top i Γ1 ρ1 Γ2 ρ2 ->
+    wf_env ρ2.
+  Proof.
+    unfold G_top.
+    intros; tauto.
+  Qed.
+
+  Lemma G_top_subset i Γ1 ρ1 Γ2 ρ2 Γ3 Γ4 :
+    G_top i Γ1 ρ1 Γ2 ρ2 ->
+    Γ3 \subset Γ1 ->
+    Γ4 \subset Γ3 ->
+    G_top i Γ3 ρ1 Γ4 ρ2.
+  Proof.
+    unfold G_top.
+    intros.
+    destruct H as [Hr [Hs HG]].
+    repeat (split; auto).
+  Qed.
+
+  Lemma G_top_G : forall {i Γ1 ρ1 Γ2 ρ2},
       G_top i Γ1 ρ1 Γ2 ρ2 ->
-      wf_env ρ2.
-    Proof.
-      unfold G_top.
-      intros; tauto.
-    Qed.
+      G i Γ1 ρ1 Γ2 ρ2.
+  Proof.
+    unfold G_top, G.
+    intros.
+    destruct H as [HΓ [Hρ HG]].
+    unfold Ensembles.Included, Ensembles.In, Dom_map in *.
+    split; auto; intros.
+    edestruct HG as [v1' [v2 [Heqv1 [Heqv2 [Hex HV]]]]]; eauto.
+    rewrite Heqv1 in H0; inv H0; eauto.
+  Qed.
 
-    Lemma G_top_subset i Γ1 ρ1 Γ2 ρ2 Γ3 Γ4 :
-      G_top i Γ1 ρ1 Γ2 ρ2 ->
-      Γ3 \subset Γ1 ->
-      Γ4 \subset Γ3 ->
-      G_top i Γ3 ρ1 Γ4 ρ2.
-    Proof.
-      unfold G_top.
-      intros.
-      destruct H as [Hr [Hs HG]].
-      repeat (split; auto).
-    Qed.
+End Spec.
 
-    Lemma G_top_G : forall {i Γ1 ρ1 Γ2 ρ2},
-        G_top i Γ1 ρ1 Γ2 ρ2 ->
-        G i Γ1 ρ1 Γ2 ρ2.
-    Proof.
-      unfold G_top, G.
-      intros.
-      destruct H as [HΓ [Hρ HG]].
-      unfold Ensembles.Included, Ensembles.In, Dom_map in *.
-      split; auto; intros.
-      edestruct HG as [v1' [v2 [Heqv1 [Heqv2 [Hex HV]]]]]; eauto.
-      rewrite Heqv1 in H0; inv H0; eauto.
-    Qed.
-
-  End Spec.
-
-  Definition trans_correct_top etop etop' :=
-    A1.occurs_free etop' \subset A0.occurs_free etop /\
+Definition trans_correct_top etop etop' :=
+  A1.occurs_free etop' \subset A0.occurs_free etop /\
     forall i ρ1 ρ2,
       let K := analyze etop in
       G_top K i (A0.occurs_free etop) ρ1 (A1.occurs_free etop') ρ2 ->
